feat: add reasoning principle for for loops

CoqOfNoir/simulation/CoqOfNoir.v
@@ -1,34 +1,44 @@
 Require Import CoqOfNoir.CoqOfNoir.
 
+Module ToValue.
+  Class Trait (Self : Set) : Set := {
+    to_value : Self -> Value.t;
+  }.
+End ToValue.
+Export ToValue.
+
 Module Panic.
   Inductive t (A : Set) : Set :=
-  | Value : A -> t A
-  (** The [Panic] works with an existential type, so we can return any payload for errors. This is
-      useful for debugging. Then we cannot catch the error and compute with it as we do not know the
-      type anymore, but catching panic errors is not supposed to happen in Rust. *)
-  | Panic (payload : {Error : Set @ Error}) : t A.
-  Arguments Value {_}.
-  Arguments Panic {_}.
+  | Success : A -> t A
+  (** We put the payload on the parameter on a smart contructor, that is actually an opaque function
+      that forgets about its parameter. *)
+  | Error : t A.
+  Arguments Success {_}.
+  Arguments Error {_}.
+
+  Definition to_result {A : Set} `{ToValue.Trait A} (value : t A) : Result.t :=
+    match value with
+    | Success value => Result.Ok (to_value value)
+    | Error => Result.Panic
+    end.
 
   Definition return_ {A : Set} (value : A) : t A :=
-    Value value.
+    Success value.
+  Arguments return_ /.
 
-  Definition panic {A Error : Set} (error : Error) : t A :=
-    Panic (existS _ error).
+  Definition panic {A E : Set} (error : E) : t A :=
+    Error.
+  (* So that the error payload appears for debugging *)
+  Opaque panic.
 
   Definition bind {A B : Set} (value : t A) (f : A -> t B) : t B :=
     match value with
-    | Value value => f value
-    | Panic error => Panic error
+    | Success value => f value
+    | Error => Error
     end.
 
   Definition fold_left {A B : Set} (init : A) (l : list B) (f : A -> B -> t A) : t A :=
     List.fold_left (fun acc x => bind acc (fun acc => f acc x)) l (return_ init).
-
-  Definition map {A B : Set} (l : list A) (f : A -> t B) : t (list B) :=
-    List.fold_right
-      (fun x acc => bind acc (fun acc => bind (f x) (fun x => return_ (x :: acc))))
-      (return_ []) l.
 End Panic.
 
 Module PanicNotations.
@@ -46,18 +56,56 @@ Module PanicNotations.
     (at level 200, X at level 100, Y at level 200).
 
   Notation "fold!" := Panic.fold_left.
-
-  Notation "map!" := Panic.map.
 End PanicNotations.
 
-Export PanicNotations.
+Module StatePanic.
+  Definition t (State : Set) (A : Set) : Set :=
+    State -> Panic.t A * State.
 
-Module ToValue.
-  Class Trait (Self : Set) : Set := {
-    to_value : Self -> Value.t;
-  }.
-End ToValue.
-Export ToValue.
+  Definition return_ {State A : Set} (value : A) : t State A :=
+    fun state => (Panic.return_ value, state).
+
+  Definition bind {State A B : Set} (value : t State A) (f : A -> t State B) : t State B :=
+    fun state =>
+      let '(output, state) := value state in
+      match output with
+      | Panic.Success value => f value state
+      | Panic.Error => (Panic.Error, state)
+      end.
+
+  Fixpoint fold_left {State A B : Set}
+      (init : A) (l : list B) (f : A -> B -> t State A) {struct l} :
+      t State A :=
+    match l with
+    | [] => return_ init
+    | x :: l => bind (f init x) (fun init => fold_left init l f)
+    end.
+End StatePanic.
+
+Module StatePanicNotations.
+  Notation "MS!" := StatePanic.t.
+
+  Notation "returnS!" := StatePanic.return_.
+  Notation "panic!" := Panic.panic.
+
+  Notation "'letS!' x ':=' X 'in' Y" :=
+    (StatePanic.bind X (fun x => Y))
+    (at level 200, x pattern, X at level 100, Y at level 200).
+
+  Notation "'doS!' X 'in' Y" :=
+    (StatePanic.bind X (fun (_ : unit) => Y))
+    (at level 200, X at level 100, Y at level 200).
+
+  Notation "foldS!" := StatePanic.fold_left.
+End StatePanicNotations.
+
+Export PanicNotations.
+Export StatePanicNotations.
+
+Global Instance Impl_ToValue_for_unit : ToValue.Trait unit := {
+  to_value (_ : unit) :=
+    Value.Tuple [];
+}.
 
 Global Instance Impl_ToValue_for_bool : ToValue.Trait bool := {
   to_value (b : bool) :=
@@ -65,123 +113,123 @@ Global Instance Impl_ToValue_for_bool : ToValue.Trait bool := {
 }.
 
 Module Field.
-  Inductive t : Set :=
-  | Make (z : Z).
+  Record t : Set := {
+    value : Z;
+  }.
 
   Global Instance Impl_ToValue : ToValue.Trait t := {
     to_value (i : t) :=
-      let 'Make i := i in
-      Value.Integer IntegerKind.Field i;
+      Value.Integer IntegerKind.Field i.(value);
   }.
 End Field.
 
 Module U1.
-  Inductive t : Set :=
-  | Make (i : Z).
+  Record t : Set := {
+    value : Z;
+  }.
 
   Global Instance Impl_ToValue : ToValue.Trait t := {
     to_value (i : t) :=
-      let 'Make i := i in
-      Value.Integer IntegerKind.U1 i;
+      Value.Integer IntegerKind.U1 i.(value);
   }.
 End U1.
 
 Module U8.
-  Inductive t : Set :=
-  | Make (z : Z).
+  Record t : Set := {
+    value : Z;
+  }.
 
   Global Instance Impl_ToValue : ToValue.Trait t := {
     to_value (i : t) :=
-      let 'Make i := i in
-      Value.Integer IntegerKind.U8 i;
+      Value.Integer IntegerKind.U8 i.(value);
   }.
 End U8.
 
 Module U16.
-  Inductive t : Set :=
-  | Make (z : Z).
+  Record t : Set := {
+    value : Z;
+  }.
 
   Global Instance Impl_ToValue : ToValue.Trait t := {
     to_value (i : t) :=
-      let 'Make i := i in
-      Value.Integer IntegerKind.U16 i;
+      Value.Integer IntegerKind.U16 i.(value);
   }.
 End U16.
 
 Module U32.
-  Inductive t : Set :=
-  | Make (z : Z).
+  Record t : Set := {
+    value : Z;
+  }.
 
   Global Instance Impl_ToValue : ToValue.Trait t := {
     to_value (i : t) :=
-      let 'Make i := i in
-      Value.Integer IntegerKind.U32 i;
+      Value.Integer IntegerKind.U32 i.(value);
   }.
 End U32.
 
 Module U64.
-  Inductive t : Set :=
-  | Make (z : Z).
+  Record t : Set := {
+    value : Z;
+  }.
 
   Global Instance Impl_ToValue : ToValue.Trait t := {
     to_value (i : t) :=
-      let 'Make i := i in
-      Value.Integer IntegerKind.U64 i;
+      Value.Integer IntegerKind.U64 i.(value);
   }.
 End U64.
 
 Module I1.
-  Inductive t : Set :=
-  | Make (z : Z).
+  Record t : Set := {
+    value : Z;
+  }.
 
   Global Instance Impl_ToValue : ToValue.Trait t := {
     to_value (i : t) :=
-      let 'Make i := i in
-      Value.Integer IntegerKind.I1 i;
+      Value.Integer IntegerKind.I1 i.(value);
   }.
 End I1.
 
 Module I8.
-  Inductive t : Set :=
-  | Make (z : Z).
+  Record t : Set := {
+    value : Z;
+  }.
 
   Global Instance Impl_ToValue : ToValue.Trait t := {
     to_value (i : t) :=
-      let 'Make i := i in
-      Value.Integer IntegerKind.I8 i;
+      Value.Integer IntegerKind.I8 i.(value);
   }.
 End I8.
 
 Module I16.
-  Inductive t : Set :=
-  | Make (z : Z).
+  Record t : Set := {
+    value : Z;
+  }.
 
   Global Instance Impl_ToValue : ToValue.Trait t := {
     to_value (i : t) :=
-      let 'Make i := i in
-      Value.Integer IntegerKind.I16 i;
+      Value.Integer IntegerKind.I16 i.(value);
   }.
 End I16.
 
 Module I32.
-  Inductive t : Set :=
-  | Make (z : Z).
+  Record t : Set := {
+    value : Z;
+  }.
 
   Global Instance Impl_ToValue : ToValue.Trait t := {
     to_value (i : t) :=
-      let 'Make i := i in
-      Value.Integer IntegerKind.I32 i;
+      Value.Integer IntegerKind.I32 i.(value);
   }.
 End I32.
 
 Module I64.
-  Inductive t : Set :=
-  | Make (z : Z).
+  Record t : Set := {
+    value : Z;
+  }.
 
   Global Instance Impl_ToValue : ToValue.Trait t := {
     to_value (i : t) :=
-      let 'Make i := i in
-      Value.Integer IntegerKind.I64 i;
+      Value.Integer IntegerKind.I64 i.(value);
   }.
 End I64.
 
@@ -193,68 +241,57 @@ End SemiInteger.
 
 Global Instance Impl_SemiInteger_for_Field : SemiInteger.Trait Field.t := {
   SemiInteger.to_Z (i : Field.t) :=
-    let 'Field.Make i := i in
-    i;
+    i.(Field.value);
 }.
 
 Global Instance Impl_SemiInteger_for_U1 : SemiInteger.Trait U1.t := {
   SemiInteger.to_Z (i : U1.t) :=
-    let 'U1.Make i := i in
-    i;
+    i.(U1.value);
 }.
 
 Global Instance Impl_SemiInteger_for_U8 : SemiInteger.Trait U8.t := {
   SemiInteger.to_Z (i : U8.t) :=
-    let 'U8.Make i := i in
-    i;
+    i.(U8.value);
 }.
 
 Global Instance Impl_SemiInteger_for_U16 : SemiInteger.Trait U16.t := {
   SemiInteger.to_Z (i : U16.t) :=
-    let 'U16.Make i := i in
-    i;
+    i.(U16.value);
 }.
 
 Global Instance Impl_SemiInteger_for_U32 : SemiInteger.Trait U32.t := {
   SemiInteger.to_Z (i : U32.t) :=
-    let 'U32.Make i := i in
-    i;
+    i.(U32.value);
 }.
 
 Global Instance Impl_SemiInteger_for_U64 : SemiInteger.Trait U64.t := {
   SemiInteger.to_Z (i : U64.t) :=
-    let 'U64.Make i := i in
-    i;
+    i.(U64.value);
 }.
 
 Global Instance Impl_SemiInteger_for_I1 : SemiInteger.Trait I1.t := {
   SemiInteger.to_Z (i : I1.t) :=
-    let 'I1.Make i := i in
-    i;
+    i.(I1.value);
 }.
 
 Global Instance Impl_SemiInteger_for_I8 : SemiInteger.Trait I8.t := {
   SemiInteger.to_Z (i : I8.t) :=
-    let 'I8.Make i := i in
-    i;
+    i.(I8.value);
 }.
 
 Global Instance Impl_SemiInteger_for_I16 : SemiInteger.Trait I16.t := {
   SemiInteger.to_Z (i : I16.t) :=
-    let 'I16.Make i := i in
-    i;
+    i.(I16.value);
 }.
 
 Global Instance Impl_SemiInteger_for_I32 : SemiInteger.Trait I32.t := {
   SemiInteger.to_Z (i : I32.t) :=
-    let 'I32.Make i := i in
-    i;
+    i.(I32.value);
 }.
 
 Global Instance Impl_SemiInteger_for_I64 : SemiInteger.Trait I64.t := {
   SemiInteger.to_Z (i : I64.t) :=
-    let 'I64.Make i := i in
-    i;
+    i.(I64.value);
 }.
 
 Module Integer.
@@ -289,86 +326,92 @@ End Integer.
 
 Global Instance Impl_Integer_for_U1 : Integer.Trait U1.t := {
   Integer.of_Z (i : Z) :=
-    U1.Make (i mod (2^1));
+    U1.Build_t (i mod (2^1));
 }.
 
 Global Instance Impl_Integer_for_U8 : Integer.Trait U8.t := {
   Integer.of_Z (i : Z) :=
-    U8.Make (i mod (2^8));
+    U8.Build_t (i mod (2^8));
 }.
 
 Global Instance Impl_Integer_for_U16 : Integer.Trait U16.t := {
   Integer.of_Z (i : Z) :=
-    U16.Make (i mod (2^16));
+    U16.Build_t (i mod (2^16));
 }.
 
 Global Instance Impl_Integer_for_U32 : Integer.Trait U32.t := {
   Integer.of_Z (i : Z) :=
-    U32.Make (i mod (2^32));
+    U32.Build_t (i mod (2^32));
 }.
 
 Global Instance Impl_Integer_for_U64 : Integer.Trait U64.t := {
   Integer.of_Z (i : Z) :=
-    U64.Make (i mod (2^64));
+    U64.Build_t (i mod (2^64));
 }.
 
 Global Instance Impl_Integer_for_I1 : Integer.Trait I1.t := {
   Integer.of_Z (i : Z) :=
-    I1.Make (((i + 2^0) mod (2^1)) - 2^0);
+    I1.Build_t (((i + 2^0) mod (2^1)) - 2^0);
 }.
 
 Global Instance Impl_Integer_for_I8 : Integer.Trait I8.t := {
   Integer.of_Z (i : Z) :=
-    I8.Make (((i + 2^7) mod (2^8)) - 2^7);
+    I8.Build_t (((i + 2^7) mod (2^8)) - 2^7);
 }.
 
 Global Instance Impl_Integer_for_I16 : Integer.Trait I16.t := {
   Integer.of_Z (i : Z) :=
-    I16.Make (((i + 2^15) mod (2^16)) - 2^15);
+    I16.Build_t (((i + 2^15) mod (2^16)) - 2^15);
 }.
 
 Global Instance Impl_Integer_for_I32 : Integer.Trait I32.t := {
   Integer.of_Z (i : Z) :=
-    I32.Make (((i + 2^31) mod (2^32)) - 2^31);
+    I32.Build_t (((i + 2^31) mod (2^32)) - 2^31);
 }.
 
 Global Instance Impl_Integer_for_I64 : Integer.Trait I64.t := {
   Integer.of_Z (i : Z) :=
-    I64.Make (((i + 2^63) mod (2^64)) - 2^63);
+    I64.Build_t (((i + 2^63) mod (2^64)) - 2^63);
 }.
 
 Module Array.
   (** We keep the [size] explicit even if this is not needed as we represent things with a list. We
       use it as a marker to guide the type-classes inference mechanism as this is done in Noir. *)
-  Inductive t (A : Set) (size : U32.t) : Set :=
-  | Make (array : list A).
-  Arguments Make {_ _}.
+  Record t {A : Set} {size : U32.t} : Set := {
+    value : list A;
+  }.
+  Arguments t : clear implicits.
+  Arguments Build_t {_ _}.
+
+  Module Valid.
+    Definition t {A : Set} {size : U32.t} (array : t A size) : Prop :=
+      List.length array.(value) = Z.to_nat (SemiInteger.to_Z size).
+  End Valid.
 
   Global Instance Impl_ToValue {A : Set} `{ToValue.Trait A} {size : U32.t} :
       ToValue.Trait (t A size) := {
     to_value (array : t A size) :=
-      let 'Make array := array in
-      Value.Array (List.map to_value array);
+      Value.Array (List.map to_value array.(value));
   }.
 
   Definition repeat {A : Set} (size : U32.t) (value : A) : t A size :=
-    Make (List.repeat value (Z.to_nat (SemiInteger.to_Z size))).
+    {|
+      value := List.repeat value (Z.to_nat (SemiInteger.to_Z size))
+    |}.
 
   Definition read {A Index: Set} `{SemiInteger.Trait Index} {size : U32.t}
       (array : t A size) (index : Index) :
       M! A :=
-    let 'Make array := array in
-    match List.nth_error array (Z.to_nat (SemiInteger.to_Z index)) with
+    match List.nth_error array.(value) (Z.to_nat (SemiInteger.to_Z index)) with
     | Some result => return! result
     | None => panic! ("Array.get: index out of bounds", array, index)
     end.
 
   Definition write {A Index: Set} `{SemiInteger.Trait Index} {size : U32.t}
-      (array : t A size) (index : Index) (value : A) :
+      (array : t A size) (index : Index) (update : A) :
       M! (t A size) :=
-    let 'Make array := array in
-    match List.listUpdate_error array (Z.to_nat (SemiInteger.to_Z index)) value with
-    | Some array => return! (Make array)
+    match List.listUpdate_error array.(value) (Z.to_nat (SemiInteger.to_Z index)) update with
+    | Some array => return! (Build_t array)
     | None => panic! ("Array.write: index out of bounds", array, index)
     end.
 End Array.
@@ -381,15 +424,11 @@ End Eq.
 
 Global Instance Impl_Eq_for_U8 : Eq.Trait U8.t := {
   Eq.eq (self other : U8.t) :=
-    let 'U8.Make self := self in
-    let 'U8.Make other := other in
-    self =? other;
+    self.(U8.value) =? other.(U8.value);
 }.
 
 Global Instance Impl_Eq_for_Array {A : Set} `{Eq.Trait A} {size : U32.t} :
     Eq.Trait (Array.t A size) := {
   Eq.eq (self other : Array.t A size) :=
-    let 'Array.Make self := self in
-    let 'Array.Make other := other in
-    List.fold_left andb (List.zip Eq.eq self other) true;
+    List.fold_left andb (List.zip Eq.eq self.(Array.value) other.(Array.value)) true;
 }.
